Improve process_example

Coq/VeracityLogic.v
@@ -1247,26 +1247,24 @@ Definition trustV := Trust _V_.
 
 Eval compute in showForProofTree_judgement [] [(e1 \by a1 \in c1)] (e1 \by a1 \in c1) (assume _e1_ a1 c1).
 
+Definition j1 := l \by P \in c1.
+Definition j2 := s \by P \in c2.
+Definition j3 := c \by P \in c3.
+
+
 Definition process_example : proofTreeOf_wrapped P (c3 ->' (c2 ->' (c1 ->' (c1 /\' c2 /\' c3)))).
 Proof.
 eexists  _ _.
-eapply (impl_intro _c_ _ _ _ _ [(AtomicEvid _c_) \by P \in c3] [] _ _ _).
-eapply (impl_intro _s_ _ _ _ _ [(AtomicEvid _c_) \by P \in c3;(AtomicEvid _s_) \by P \in c2] [(AtomicEvid _c_) \by P \in c3] _ _ _).
-eapply (impl_intro _l_ _ _ _ _ 
-  [(AtomicEvid _l_) \by P \in c1;
-   (AtomicEvid _s_) \by P \in c2; 
-   (AtomicEvid _c_) \by P \in c3]
-   
-  [(AtomicEvid _c_) \by P \in c3;
-   (AtomicEvid _s_) \by P \in c2] _ _ _).
-eapply (and_intro _ _ _ _ _ [(AtomicEvid _l_) \by P \in c1;
-(AtomicEvid _s_) \by P \in c2] _ _ _).
+eapply (impl_intro _c_) with (Ps := [j3]) (Qs:=[]). 1,2,3: shelve.
+eapply (impl_intro _s_) with (Ps := [j2;j3]) (Qs:=[j3]). 1,2,3: shelve.
+eapply (impl_intro _l_) with (Ps := [j1;j2;j3]) (Qs:=[j2;j3]). 1,2,3: shelve.
+eapply (and_intro _ _ _ _ _ [j1;j2] _ _ _).
 eapply (and_intro _ _ _ _ _ _ _ _ _).
 eapply (assume _l_).
 eapply (assume _s_).
 eapply (assume _c_).
 Unshelve.
-all: try (simpl; reflexivity).
+all: reflexivity.
 Defined.
 
 (*|
